client1 and pipe is owrking with new spec, but I dont know if kfree and kalloc actually satisfies it

VST-introduction/VSU_kalloc_kfree_definitions.v
@@ -10,32 +10,31 @@ Require Import malloc_sep.*)
 
 (** token -- could be moved to another file *)
 
-Definition my_kalloc_token (sh: share) (sz: Z) (p: val) : mpred := (* my kalloc token is a block where we can have t_run struct in it, but also something else?*)
+Definition my_kalloc_token (sh: share) (sz: Z) (p: val) (t:type) : mpred := (* my kalloc token is a block where we can have t_run struct in it, but also something else?*)
   EX v,
     !! (
-        field_compatible t_run [] p 
-        /\ malloc_compatible (sz) p
-        /\ 0 <= sizeof t_run <= sz
+        field_compatible t [] p 
+        /\ malloc_compatible sz p
+        /\ 0 <= sizeof t <= sz
         /\ writable_share sh) 
-  && ((memory_block sh (sz) (p)) * data_at sh t_run v p). (* this is the rest of the page*)
-
+  && (((*memory_block sh (sz) (p *) (data_at sh t v p))). (* this is the rest of the page*)
   
 
 (** **** Exercise: 2 stars, standard (malloc_token_properties) *)
 Lemma my_kalloc_token_valid_pointer:
-    forall (sh : share) (sz : Z) (p : val),
-      my_kalloc_token sh sz p |-- valid_pointer p.
+    forall (sh : share) (sz : Z) (p : val) (t: type),
+    0 < sizeof t ->
+    readable_share sh ->
+      my_kalloc_token sh sz p t |-- valid_pointer p.
 Proof.
-  intros. 
-    induction sz.
-  - unfold my_kalloc_token. simpl. entailer!. entailer.
-  - unfold my_kalloc_token. simpl. entailer!. entailer.
-  - unfold my_kalloc_token. entailer!. entailer. 
+  intros.
+  unfold my_kalloc_token. entailer!.
+  apply data_at_valid_ptr; try rep_lia; auto.
 Qed.
 
 Lemma  my_kalloc_token_local_facts : 
-   forall (sh : share) (sz : Z) (p : val),
-     my_kalloc_token sh sz p |-- !! malloc_compatible sz p.
+   forall (sh : share) (sz : Z) (p : val) (t:type),
+     my_kalloc_token sh sz p t |-- !! malloc_compatible sz p.
 Proof.
   intros. 
   unfold my_kalloc_token. simpl. entailer.
@@ -47,59 +46,54 @@ Qed.
 Definition Tok_APD := Build_KallocTokenAPD my_kalloc_token my_kalloc_token_valid_pointer
    my_kalloc_token_local_facts.
 
-Definition mem_mgr (gv: globals) : mpred := (* I am unsure how to access all these elements.. *)
-EX sh: share, EX ls: list val, EX xx, EX original_freelist_pointer,
+Definition mem_mgr (gv: globals) (sh : share) (ls: list val) (xx:Z) (original_freelist_pointer:val): mpred := (* I am unsure how to access all these elements.. *)
     !! (writable_share sh /\
         is_pointer_or_null original_freelist_pointer /\
               (((ls = nil) /\ original_freelist_pointer = nullval) \/ 
               ((ls <> nil) /\ isptr original_freelist_pointer))
         ) &&
-      data_at sh t_struct_kmem (Vint (Int.repr xx), original_freelist_pointer) (gv _kmem) *
-      freelistrep sh ls original_freelist_pointer.
+      (sepcon (data_at sh t_struct_kmem (Vint (Int.repr xx), original_freelist_pointer) (gv _kmem))
+      (freelistrep sh ls original_freelist_pointer)).
 
 (************ mem_mgr lemmas etc. *************)
 Lemma mem_mgr_split: 
- forall gv:globals,
-  mem_mgr gv
+ forall (gv:globals) (sh:share) (ls: list val) (xx:Z) (original_freelist_pointer:val),
+  mem_mgr gv sh ls xx original_freelist_pointer
   = 
-  EX sh: share, EX ls: list val, EX xx, EX original_freelist_pointer,
-      !! (writable_share sh /\
-          is_pointer_or_null original_freelist_pointer /\
-          (((ls = nil) /\ original_freelist_pointer = nullval) \/ ((ls <> nil) /\ isptr original_freelist_pointer))) &&
-        data_at sh t_struct_kmem (Vint (Int.repr xx), original_freelist_pointer) (gv _kmem) *
-        freelistrep sh ls original_freelist_pointer.
+  !! (writable_share sh /\
+        is_pointer_or_null original_freelist_pointer /\
+              (((ls = nil) /\ original_freelist_pointer = nullval) \/ 
+              ((ls <> nil) /\ isptr original_freelist_pointer))
+        ) &&
+      (sepcon (data_at sh t_struct_kmem (Vint (Int.repr xx), original_freelist_pointer) (gv _kmem))
+      (freelistrep sh ls original_freelist_pointer)).
 Proof.
   intros. apply pred_ext.
-  - unfold mem_mgr. Intros sh ls xx original_freelist_pointer. entailer!.
-  Exists sh ls xx original_freelist_pointer. entailer!.
-  - Intros sh ls xx original_freelist_pointer.
-  unfold mem_mgr. Exists sh ls xx original_freelist_pointer. entailer!.
+  - unfold mem_mgr. entailer!.
+  - unfold mem_mgr. entailer!.
 Qed.
 
 
 Lemma kalloc_token'_split: 
- forall  (sh: share) (sz: Z) (p: val),
- my_kalloc_token  (sh) (sz) (p)
+ forall  (sh: share) (sz: Z) (p: val) (t:type),
+ my_kalloc_token  (sh) (sz) (p) (t)
   = 
   EX v,
     !! (
-        field_compatible t_run [] p 
-        /\ malloc_compatible (sz) p
-        /\ 0 <= sizeof t_run <= sz
+        field_compatible t [] p 
+        /\ malloc_compatible sz p
+        /\ 0 <= sizeof t <= sz
         /\ writable_share sh) 
-  && ((memory_block sh (sz) (p)) * data_at sh t_run v p). 
+  && (((*memory_block sh (sz) (p *) (data_at sh t v p))).
 Proof.
   intros. apply pred_ext.
-  - unfold my_kalloc_token. entailer!. Exists v. entailer!.
+  - unfold my_kalloc_token. entailer. entailer!. Exists v. entailer!.
   - unfold my_kalloc_token. entailer!. Exists v. entailer!.
 Qed.
 
 
 
 (************ mem_mgr lemmas etc. end *************)
-
-
-
 
 
 Definition KF_APD := Build_KallocFreeAPD Tok_APD mem_mgr.
