VST-introduction/verif_client_pipe.v
@@ -11,7 +11,7 @@ Require Import VC.VSU_kalloc_kfree_definitions.
 Definition MF_ASI: funspecs := Kalloc_ASI KF_APD _kalloc1 _kfree1.
 Definition MF_imported_specs:funspecs := nil.
 Definition MF_internal_specs: funspecs := MF_ASI.
-Definition MF_globals gv : mpred:= ASI_kalloc.mem_mgr KF_APD gv.
+Definition MF_globals gv  sh ls xx original_freelist_pointer: mpred:= ASI_kalloc.mem_mgr KF_APD gv sh ls xx original_freelist_pointer.
 Definition MFVprog : varspecs. mk_varspecs client1.prog. Defined.
 Definition MFGprog: funspecs := MF_imported_specs ++ MF_internal_specs.
 
@@ -29,71 +29,103 @@ Require Import malloc_sep.*)
 
 Definition client_11_pipealloc_spec : ident * funspec :=
  DECLARE _client_11_pipealloc
- WITH (*sh : share, original_freelist_pointer:val, xx:Z, ls:list val,*) gv:globals
+ WITH sh : share, original_freelist_pointer:val, xx:Z, ls:list val, gv:globals
  PRE [ ] 
-    PROP () PARAMS() GLOBALS(gv) SEP (MF_globals gv)
+    PROP () PARAMS() GLOBALS(gv) SEP (MF_globals gv sh ls xx original_freelist_pointer)
  POST [ tvoid ] 
-    EX p: val, 
     PROP ( ) RETURN () SEP (
-        (if eq_dec p nullval then
-        emp
-        else 
-        kalloc_token' KF_APD Ews (sizeof t_struct_pipe) p *
-        pipe_rep Ews p) 
-        * MF_globals gv).
+        (if eq_dec original_freelist_pointer nullval then
+            MF_globals gv  sh ls xx original_freelist_pointer *emp
+        else
+        EX next ls',
+          (!! (next :: ls' = ls) &&
+                pipe_rep Ews original_freelist_pointer *
+                MF_globals gv  sh ls' xx next
+        )
+        )
+    ).
     
 Definition client1_spec := 
     DECLARE _client1
-    WITH new_head:val, gv:globals
+    WITH new_head:val, sh : share, original_freelist_pointer:val, xx:Z, ls:list val, gv:globals
     PRE [ tptr tvoid ]
         PROP(is_pointer_or_null new_head) 
         PARAMS (new_head) GLOBALS(gv)
         SEP (
-            MF_globals gv *
-            if eq_dec new_head nullval then emp
-            else (kalloc_token' KF_APD Ews (sizeof t_run) new_head * data_at_ Ews t_run new_head)
+            MF_globals gv  sh ls xx original_freelist_pointer *
+            (if eq_dec new_head nullval then emp
+            else (kalloc_token' KF_APD Ews (sizeof t_run) new_head t_run))
         )
     POST [ tptr tvoid ]
-        PROP( )
-        RETURN (new_head) (* we return the head like in the pop function*)
+        EX r,
+        PROP( 
+            ((new_head = nullval) /\ ( original_freelist_pointer = nullval) /\ r = nullval) \/
+            ((new_head <> nullval) /\  r = new_head) \/
+            ((new_head = nullval) /\ ( original_freelist_pointer <> nullval) /\ r = original_freelist_pointer)
+        )
+        RETURN (r) (* we return the head like in the pop function*)
         SEP (
-            MF_globals gv *
-            if eq_dec new_head nullval then emp
-            else (kalloc_token' KF_APD Ews (sizeof t_run) new_head * data_at_ Ews t_run new_head) 
+            
+            (if eq_dec new_head nullval then 
+                (if (eq_dec original_freelist_pointer nullval) then 
+                    (emp *  MF_globals gv  sh ls xx original_freelist_pointer)
+                else (
+                    (EX next ls',
+                    (!! (next :: ls' = ls) &&
+                        MF_globals gv  sh ls' xx next
+                    ) *  
+                    kalloc_token' KF_APD Ews (sizeof t_run) original_freelist_pointer t_run)))
+            else (
+                MF_globals gv  sh ls xx original_freelist_pointer* (* is this still wrong?? *)
+                kalloc_token' KF_APD Ews (sizeof t_run) new_head t_run) )
             ).
 
+                            
 (* TODO should maybe add things to MFGprog... *)
 
 Lemma body_client_11_pipealloc: semax_body MFVprog MFGprog f_client_11_pipealloc client_11_pipealloc_spec.
 Proof.
 start_function.
 forward.
-forward_call (t_struct_pipe, gv).  (* kalloc *)
-- unfold MF_globals. entailer!.
-- Intros vret. forward_if.
-    + destruct (eq_dec vret nullval); entailer!. 
-    + destruct (eq_dec vret nullval).
-        * rewrite e in H. auto_contradict.
-        * rewrite mem_mgr_split. Intros sh ls xx original_freelist_pointer.
-        forward. forward. forward. forward. Exists vret.
-        destruct (eq_dec vret nullval); auto_contradict.
+forward_call (t_struct_pipe, gv,  sh,  ls , xx,  original_freelist_pointer).  (* kalloc *)
+- unfold MF_globals. entailer!. 
+- destruct (eq_dec original_freelist_pointer nullval) eqn:e0.
+    + forward_if.
+        * rewrite e in H; auto_contradict.
+        * forward. entailer.
+    + Intros ab. forward_if.
+        *
+        rewrite mem_mgr_split. entailer. 
+        assert(isptr original_freelist_pointer). {
+        destruct original_freelist_pointer; auto_contradict.
+        - unfold is_pointer_or_null in PNoriginal_freelist_pointer. simpl in PNoriginal_freelist_pointer.
+        subst. auto_contradict.
+        - auto.
+        }
+        destruct original_freelist_pointer; auto_contradict. admit.
+        * rewrite kalloc_token'_split. Intros v. forward. forward. forward. forward. Exists (fst ab) (snd ab).
         entailer.
-        unfold pipe_rep. entailer!.
-        unfold MF_globals. rewrite mem_mgr_split. Exists sh ls xx original_freelist_pointer. entailer!.
-        apply derives_refl.
-    + forward. Exists vret. destruct (eq_dec vret nullval); auto_contradict. entailer.
-Qed.
+        unfold MF_globals. unfold pipe_rep.  Exists (fst v). entailer!.
+        * forward. entailer.
+Admitted.
 
 Lemma body_client1: semax_body MFVprog MFGprog f_client1 client1_spec.
 Proof.
 start_function. 
-forward_call (t_run, new_head , gv).  (* kfree *)
-- unfold MF_globals. entailer!. 
-destruct (eq_dec new_head nullval); entailer!. apply derives_refl.
-- forward_call (t_run, gv).  (* kalloc *)
-Intros vret. forward. (* same problem as before.. *)
-Admitted.
-
-
-
-
+forward_call (t_run, new_head, gv, sh, ls, xx:Z, original_freelist_pointer).  (* kfree *)
+    + destruct (eq_dec new_head nullval).
+        *unfold MF_globals. entailer!.
+        * unfold MF_globals. entailer!. apply derives_refl.
+    + destruct (eq_dec new_head nullval).
+        *forward_call (t_run, gv, sh, ls, xx, original_freelist_pointer).  (* kalloc *)
+        destruct (eq_dec original_freelist_pointer nullval).
+            -- forward. Exists nullval. unfold MF_globals. entailer!.
+            -- destruct ls.
+                ++ forward. auto_contradict.
+                ++ forward. Exists original_freelist_pointer. entailer. Exists v. entailer.
+                    Exists ls. entailer. unfold MF_globals. entailer!. inversion H0; subst. entailer!.
+        *forward_call (t_run, gv, sh, original_freelist_pointer::ls, xx, new_head).  (* kalloc *)
+        destruct (eq_dec new_head nullval).
+            -- forward.
+            -- forward. Exists new_head. entailer. inversion H0; subst; entailer. unfold MF_globals. entailer!.
+Qed.
