VST-introduction/ASI_kalloc.v
@@ -5,16 +5,18 @@ Require Import VC.helper.
 Global Open Scope funspec_scope.
 
 Record KallocTokenAPD := {
-  kalloc_token': share -> Z -> val -> mpred;
-  kalloc_token'_valid_pointer: forall sh sz p, 
-      kalloc_token' sh sz p |-- valid_pointer p;
+  kalloc_token': share -> Z -> val -> type -> mpred;
+  kalloc_token'_valid_pointer: forall sh sz p t, 
+  0 < sizeof t ->
+  readable_share sh ->
+      kalloc_token' sh sz p t |-- valid_pointer p;
   kalloc_token'_local_facts:  forall sh sz p, 
       kalloc_token' sh sz p |-- !! malloc_compatible sz p;
 }.
 
 Record KallocFreeAPD := {
   MF_Tok :> KallocTokenAPD;
-  mem_mgr: globals -> mpred;
+  mem_mgr: globals -> share -> list val -> Z -> val -> mpred;
 }.
 
 #[export] Hint Resolve kalloc_token'_valid_pointer : valid_pointer. 
@@ -26,46 +28,54 @@ Variable K: KallocFreeAPD.
 Variable kalloc1ID: ident.
 Variable kfree1ID: ident.
 
-
 Definition kfree1_spec := 
   DECLARE kfree1ID
-      WITH t:type, new_head:val, gv:globals 
+      WITH t:type, new_head:val, gv:globals, sh:share, ls: list val, xx:Z, original_freelist_pointer:val
       PRE [ tptr tvoid]
         PROP(
               is_pointer_or_null new_head
               ) 
         PARAMS (new_head) GLOBALS(gv)
         SEP (
-          mem_mgr K gv;
+          mem_mgr K gv sh ls xx original_freelist_pointer;
           if eq_dec new_head nullval then emp
-          else (kalloc_token' K Ews (sizeof t) new_head * data_at_ Ews t new_head)
+          else (kalloc_token' K Ews (sizeof t) new_head t (** data_at_ Ews t new_head*))
         )
       POST [ tvoid ]
         PROP()
         RETURN () 
         SEP (
-          mem_mgr K gv
+          if eq_dec new_head nullval then 
+          mem_mgr K gv sh ls xx original_freelist_pointer
+          else 
+            mem_mgr K gv sh (original_freelist_pointer::ls) xx new_head
             ).
 
 
 Definition kalloc1_spec :=
 DECLARE kalloc1ID
-WITH t:type, gv:globals 
+WITH t:type, gv:globals, sh:share, ls: list val, xx:Z, original_freelist_pointer:val
 PRE [ ]
     PROP(0 <= sizeof t <= PGSIZE;
     complete_legal_cosu_type t = true;
     natural_aligned natural_alignment t = true) 
     PARAMS () GLOBALS(gv)
-    SEP ( mem_mgr K gv )  
+    SEP ( mem_mgr K gv sh ls xx original_freelist_pointer )  
 POST [ tptr tvoid ]
-  EX p:val,
     PROP()
-    RETURN (p) 
+    RETURN (original_freelist_pointer) 
     SEP (
-      mem_mgr K gv;
-      if eq_dec p nullval then emp
-      else (kalloc_token' K Ews (sizeof t) p * data_at_ Ews t p) (** TODO: fix EWs...*)
-        ).
+      if (eq_dec original_freelist_pointer nullval) then
+      mem_mgr K gv sh ls xx original_freelist_pointer * emp
+      else 
+        (
+          EX next ls',
+          (!! (next :: ls' = ls) &&
+              kalloc_token' K Ews (sizeof t) original_freelist_pointer t *
+              mem_mgr K gv sh ls' xx next
+        )
+        )
+    ).
 
 Definition Kalloc_ASI:funspecs := [kalloc1_spec; kfree1_spec].
 End Kalloc_ASI.
